Fix a typing bug occurring when SELF was used in a Michelson origination
When type-checking the code literal of a smart contract originated
from Michelson, we have to be cautious to use the self type of the
contract being originated instead of the contract doing the
origination.

For this reason, we cannot have `self_type` as a parameter of the
inductive type for instructions but it needs to be an index.

However, SELF is forbidden inside lambdas in Michelson so we do not
have to care about typing the SELF instruction in lambdas.

src/contracts_coq/boomerang.v
@@ -38,7 +38,7 @@ End ST.
 Module boomerang(C:ContractContext)(E:Env ST C).
 Module semantics := Semantics ST C E. Import semantics.
 
-Definition boomerang : full_contract storage_ty :=
+Definition boomerang : full_contract _ ST.self_type storage_ty :=
   (
     CDR ;;
     NIL operation ;;
@@ -82,7 +82,7 @@ Qed.
 Lemma boomerang_correct :
   forall (ops : data (list operation)) (fuel : Datatypes.nat),
   fuel >= 42 ->
-  eval boomerang fuel ((tt, tt), tt) = Return _ ((ops, tt), tt)
+  eval env boomerang fuel ((tt, tt), tt) = Return _ ((ops, tt), tt)
   <->
   (amount env = (0 ~Mutez) /\ ops = nil) \/
   (amount env <> (0 ~Mutez) /\
@@ -108,7 +108,8 @@ Proof.
       intro; subst ops.
       intuition.
     + intros [(Hl, Hops)|(Hr, _)].
-      * destruct Hl; congruence.
+      * simplify_instruction.
+        subst; reflexivity.
       * symmetry in Heq.
         contradiction.
   - intro Hneq.
