src/michocoq/macros.v
@@ -22,13 +22,16 @@
 Require Import syntax.
 Require Import comparable.
 
-Module Macros(ST:SelfType)(C:ContractContext).
+Module Macros(C:ContractContext).
 
-Module syntax := Syntax ST C.
+Module syntax := Syntax C.
 Export syntax.
 
-Definition CMPop (a : comparable_type) S (op : instruction Datatypes.false (int ::: S) (bool ::: S))
-           : instruction Datatypes.false (a ::: a ::: S) (bool ::: S) := COMPARE ;; op.
+Section macros.
+  Context {self_type : Datatypes.option type}.
+
+Definition CMPop (a : comparable_type) S (op : instruction self_type Datatypes.false (int ::: S) (bool ::: S))
+           : instruction self_type Datatypes.false (a ::: a ::: S) (bool ::: S) := COMPARE ;; op.
 
 Definition CMPEQ {a S} := CMPop a S EQ.
 Definition CMPNEQ {a S} := CMPop a S NEQ.
@@ -38,8 +41,8 @@ Definition CMPLE {a S} := CMPop a S LE.
 Definition CMPGE {a S} := CMPop a S GE.
 
 Definition IFop SA SB tffa tffb
-           (bt : instruction tffa SA SB) (bf : instruction tffb SA SB)
-           (op : instruction Datatypes.false (int ::: SA) (bool ::: SA)) :=
+           (bt : instruction self_type tffa SA SB) (bf : instruction self_type tffb SA SB)
+           (op : instruction self_type Datatypes.false (int ::: SA) (bool ::: SA)) :=
   op ;; IF_ bt bf.
 
 Definition IFEQ {SA SB tffa tffb} bt bf := IFop SA SB tffa tffb bt bf EQ.
@@ -50,9 +53,9 @@ Definition IFLE {SA SB tffa tffb} bt bf := IFop SA SB tffa tffb bt bf LE.
 Definition IFGE {SA SB tffa tffb} bt bf := IFop SA SB tffa tffb bt bf GE.
 
 Definition IFCMPop (a : comparable_type) SA SB tffa tffb
-           (bt : instruction tffa SA SB) (bf : instruction tffb SA SB)
-           (op : instruction Datatypes.false (int ::: SA) (bool ::: SA)) :
-  instruction (tffa && tffb) (a ::: a ::: SA) SB :=
+           (bt : instruction self_type tffa SA SB) (bf : instruction self_type tffb SA SB)
+           (op : instruction self_type Datatypes.false (int ::: SA) (bool ::: SA)) :
+  instruction self_type (tffa && tffb) (a ::: a ::: SA) SB :=
   COMPARE ;; op ;; IF_ bt bf.
 
 Definition IFCMPEQ {a SA SB tffa tffb} bt bf := IFCMPop a SA SB tffa tffb bt bf EQ.
@@ -62,11 +65,11 @@ Definition IFCMPGT {a SA SB tffa tffb} bt bf := IFCMPop a SA SB tffa tffb bt bf 
 Definition IFCMPLE {a SA SB tffa tffb} bt bf := IFCMPop a SA SB tffa tffb bt bf LE.
 Definition IFCMPGE {a SA SB tffa tffb} bt bf := IFCMPop a SA SB tffa tffb bt bf GE.
 
-Definition FAIL {SA SB} : instruction Datatypes.true SA SB := UNIT ;; FAILWITH.
+Definition FAIL {SA SB} : instruction self_type Datatypes.true SA SB := UNIT ;; FAILWITH.
 
-Definition ASSERT {S} : instruction Datatypes.false (bool ::: S) S := IF_ NOOP FAIL.
+Definition ASSERT {S} : instruction self_type Datatypes.false (bool ::: S) S := IF_ NOOP FAIL.
 
-Definition ASSERT_op S (op : instruction Datatypes.false (int ::: S) (bool ::: S)) : instruction Datatypes.false (int ::: S) S :=
+Definition ASSERT_op S (op : instruction self_type Datatypes.false (int ::: S) (bool ::: S)) : instruction self_type Datatypes.false (int ::: S) S :=
   IFop _ _ _ _ NOOP FAIL op.
 
 Definition ASSERT_EQ {S} := ASSERT_op S EQ.
@@ -76,8 +79,8 @@ Definition ASSERT_GT {S} := ASSERT_op S GT.
 Definition ASSERT_LE {S} := ASSERT_op S LE.
 Definition ASSERT_GE {S} := ASSERT_op S GE.
 
-Definition ASSERT_CMPop (a : comparable_type) S (op : instruction Datatypes.false (int ::: S) (bool ::: S))
-  : instruction Datatypes.false (a ::: a ::: S) S := IFCMPop _ _ _ _ _ NOOP FAIL op.
+Definition ASSERT_CMPop (a : comparable_type) S (op : instruction self_type Datatypes.false (int ::: S) (bool ::: S))
+  : instruction self_type Datatypes.false (a ::: a ::: S) S := IFCMPop _ _ _ _ _ NOOP FAIL op.
 
 Definition ASSERT_CMPEQ {a S} := ASSERT_CMPop a S EQ.
 Definition ASSERT_CMPNEQ {a S} := ASSERT_CMPop a S NEQ.
@@ -86,79 +89,79 @@ Definition ASSERT_CMPGT {a S} := ASSERT_CMPop a S GT.
 Definition ASSERT_CMPLE {a S} := ASSERT_CMPop a S LE.
 Definition ASSERT_CMPGE {a S} := ASSERT_CMPop a S GE.
 
-Definition ASSERT_NONE {a S} : instruction Datatypes.false (option a ::: S) S :=
+Definition ASSERT_NONE {a S} : instruction self_type Datatypes.false (option a ::: S) S :=
   IF_NONE NOOP FAIL.
 
-Definition ASSERT_SOME {a S} : instruction Datatypes.false (option a ::: S) (a ::: S) :=
+Definition ASSERT_SOME {a S} : instruction self_type Datatypes.false (option a ::: S) (a ::: S) :=
   IF_NONE FAIL NOOP.
 
-Definition ASSERT_LEFT {a b S} : instruction Datatypes.false (or a b ::: S) (a ::: S) :=
+Definition ASSERT_LEFT {a b S} : instruction self_type Datatypes.false (or a b ::: S) (a ::: S) :=
   IF_LEFT NOOP FAIL.
-Definition ASSERT_RIGHT {a b S} : instruction Datatypes.false (or a b ::: S) (b ::: S) :=
+Definition ASSERT_RIGHT {a b S} : instruction self_type Datatypes.false (or a b ::: S) (b ::: S) :=
   IF_LEFT FAIL NOOP.
 
-Definition DROP1 {a SA} : instruction Datatypes.false (a ::: SA) SA :=
+Definition DROP1 {a SA} : instruction self_type Datatypes.false (a ::: SA) SA :=
   DROP (A := a ::: nil) 1 eq_refl.
 
-Definition DIP1 {a SA SB} code : instruction _ (a ::: SA) (a ::: SB) :=
+Definition DIP1 {a SA SB} code : instruction self_type _ (a ::: SA) (a ::: SB) :=
   DIP (A := (a ::: nil)) 1 eq_refl code.
-Definition DIIP {a b SA SB} code : instruction _ (a ::: b ::: SA) (a ::: b ::: SB) :=
+Definition DIIP {a b SA SB} code : instruction self_type _ (a ::: b ::: SA) (a ::: b ::: SB) :=
   DIP (A := (a ::: b ::: nil)) 2 eq_refl code.
 Definition DIIIP {a b c SA SB} code :
-  instruction _ (a ::: b ::: c ::: SA) (a ::: b ::: c ::: SB) :=
+  instruction self_type _ (a ::: b ::: c ::: SA) (a ::: b ::: c ::: SB) :=
   DIP (A := (a ::: b ::: c ::: nil)) 3 eq_refl code.
 Definition DIIIIP {a b c d SA SB} code :
-  instruction _ (a ::: b ::: c ::: d ::: SA) (a ::: b ::: c ::: d ::: SB) :=
+  instruction self_type _ (a ::: b ::: c ::: d ::: SA) (a ::: b ::: c ::: d ::: SB) :=
   DIP (A := (a ::: b ::: c ::: d ::: nil)) 4 eq_refl code.
 
-Definition DUUP {a b S} : instruction Datatypes.false (a ::: b ::: S) (b ::: a ::: b ::: S) :=
+Definition DUUP {a b S} : instruction self_type Datatypes.false (a ::: b ::: S) (b ::: a ::: b ::: S) :=
   DIP1 DUP ;; SWAP.
 
-Definition DUPn {A b C} n (H : length A = n) : instruction Datatypes.false (A +++ b ::: C) (b ::: A +++ b ::: C) :=
+Definition DUPn {A b C} n (H : length A = n) : instruction self_type Datatypes.false (A +++ b ::: C) (b ::: A +++ b ::: C) :=
   DIG n H ;; DUP ;; DIP1 (DUG n H).
 
-Definition DUUUP {a b c S} : instruction Datatypes.false (a ::: b ::: c ::: S) (c ::: a ::: b ::: c ::: S) :=
+Definition DUUUP {a b c S} : instruction self_type Datatypes.false (a ::: b ::: c ::: S) (c ::: a ::: b ::: c ::: S) :=
   DUPn (A := a ::: b ::: nil) 2 eq_refl.
 
-Definition DUUUUP {a b c d S} : instruction Datatypes.false (a ::: b ::: c ::: d ::: S) (d ::: a ::: b ::: c ::: d ::: S) :=
+Definition DUUUUP {a b c d S} : instruction self_type Datatypes.false (a ::: b ::: c ::: d ::: S) (d ::: a ::: b ::: c ::: d ::: S) :=
   DUPn (A := a ::: b ::: c ::: nil) 3 eq_refl.
 
 (* Missing: PAPPAIIR and such *)
 
-Definition UNPAIR {a b S} : instruction Datatypes.false (pair a b ::: S) (a ::: b ::: S) :=
+Definition UNPAIR {a b S} : instruction self_type Datatypes.false (pair a b ::: S) (a ::: b ::: S) :=
   DUP ;; CAR ;; DIP1 CDR.
 
-Definition CAAR {a b c S} : instruction Datatypes.false (pair (pair a b) c ::: S) (a ::: S) :=
+Definition CAAR {a b c S} : instruction self_type Datatypes.false (pair (pair a b) c ::: S) (a ::: S) :=
   CAR ;; CAR.
 
-Definition CADR {a b c S} : instruction Datatypes.false (pair (pair a b) c ::: S) (b ::: S) :=
+Definition CADR {a b c S} : instruction self_type Datatypes.false (pair (pair a b) c ::: S) (b ::: S) :=
   CAR ;; CDR.
 
-Definition CDAR {a b c S} : instruction Datatypes.false (pair a (pair b c) ::: S) (b ::: S) :=
+Definition CDAR {a b c S} : instruction self_type Datatypes.false (pair a (pair b c) ::: S) (b ::: S) :=
   CDR ;; CAR.
 
-Definition CDDR {a b c S} : instruction Datatypes.false (pair a (pair b c) ::: S) (c ::: S) :=
+Definition CDDR {a b c S} : instruction self_type Datatypes.false (pair a (pair b c) ::: S) (c ::: S) :=
   CDR ;; CDR.
 
-Definition IF_SOME {a SA SB tffa tffb} (bt : instruction tffa _ _) (bf : instruction tffb _ _) : instruction _ (option a ::: SA) SB :=
+Definition IF_SOME {a SA SB tffa tffb} (bt : instruction self_type tffa _ _) (bf : instruction self_type tffb _ _) : instruction self_type _ (option a ::: SA) SB :=
   IF_NONE bf bt.
 
-Definition SET_CAR {a b S} : instruction Datatypes.false (pair a b ::: a ::: S) (pair a b ::: S) :=
+Definition SET_CAR {a b S} : instruction self_type Datatypes.false (pair a b ::: a ::: S) (pair a b ::: S) :=
   CDR ;; SWAP ;; PAIR.
 
-Definition SET_CDR {a b S} : instruction Datatypes.false (pair a b ::: b ::: S) (pair a b ::: S) :=
+Definition SET_CDR {a b S} : instruction self_type Datatypes.false (pair a b ::: b ::: S) (pair a b ::: S) :=
   CAR ;; PAIR.
 
-Definition MAP_CAR {a1 a2 b S} (code : instruction Datatypes.false (a1 ::: S) (a2 ::: S)) :
-  instruction Datatypes.false (pair a1 b ::: S) (pair a2 b ::: S) :=
+Definition MAP_CAR {a1 a2 b S} (code : instruction self_type Datatypes.false (a1 ::: S) (a2 ::: S)) :
+  instruction self_type Datatypes.false (pair a1 b ::: S) (pair a2 b ::: S) :=
   DUP ;; CDR ;; DIP1 (CAR ;; code) ;; SWAP ;; PAIR.
 
-Definition MAP_CDR {a b1 b2 S} (code : instruction Datatypes.false (b1 ::: pair a b1 ::: S) (b2 ::: pair a b1 ::: S)) :
-  instruction Datatypes.false (pair a b1 ::: S) (pair a b2 ::: S) :=
+Definition MAP_CDR {a b1 b2 S} (code : instruction self_type Datatypes.false (b1 ::: pair a b1 ::: S) (b2 ::: pair a b1 ::: S)) :
+  instruction self_type Datatypes.false (pair a b1 ::: S) (pair a b2 ::: S) :=
   DUP ;; CDR ;; code ;; SWAP ;; CAR ;; PAIR.
 
 
-Definition UNPAPAIR {a b c S} : instruction Datatypes.false (pair a (pair b c) :: S) (a ::: b ::: c ::: S) := UNPAIR ;; DIP1 UNPAIR.
-Definition PAPAIR {a b c S} : instruction Datatypes.false (a ::: b ::: c ::: S) (pair a (pair b c) :: S) := DIP1 PAIR;; PAIR.
-
+Definition UNPAPAIR {a b c S} : instruction self_type Datatypes.false (pair a (pair b c) :: S) (a ::: b ::: c ::: S) := UNPAIR ;; DIP1 UNPAIR.
+Definition PAPAIR {a b c S} : instruction self_type Datatypes.false (a ::: b ::: c ::: S) (pair a (pair b c) :: S) := DIP1 PAIR;; PAIR.
+End macros.
 End Macros.
